try composing API functions

src/Bedrock/API.v
@@ -18,12 +18,16 @@ Import AbstractInterpretation.Compilers.
 Import Language.Wf.Compilers.
 
 Class bedrock2_unsaturated_solinas p n s c :=
-  { carry_mul : bedrock_func;
-    spec_of_carry_mul : spec_of (fst carry_mul) :=
-      @spec_of_carry_mul p n s c (fst carry_mul);
+  { carry_mul_name : string;
+    carry_mul_func : (list string * list string * cmd)%type;
+    carry_mul : bedrock_func := (carry_mul_name, carry_mul_func);
+    spec_of_carry_mul : spec_of carry_mul_name :=
+      @spec_of_carry_mul p n s c carry_mul_name;
     carry_mul_correct :
       forall functions,
         spec_of_carry_mul (carry_mul :: functions) }.
+Arguments carry_mul_name {_ _ _ _ _}.
+Arguments carry_mul_func {_ _ _ _ _}.
 Arguments carry_mul {_ _ _ _ _}.
 Arguments spec_of_carry_mul {_ _ _ _ _}.
 Arguments carry_mul_correct {_ _ _ _ _}.
@@ -106,21 +110,23 @@ Ltac make_all_reified_ops n s c machine_wordsize :=
     n (PushButtonSynthesis.UnsaturatedSolinas.carry_mul
          n s c machine_wordsize).
 
-Ltac instantiate_ops carry_mul_name :=
+Ltac instantiate_ops carry_mul_name_value :=
   let n :=
       lazymatch goal with
       | |- bedrock2_unsaturated_solinas _ ?n _ _ => n end in
-  let carry_mul_func := fresh "carry_mul_func" in
+  let carry_mul_func_value := fresh "carry_mul_func" in
   let carry_mul_func_eq := fresh "carry_mul_func_eq" in
   lazymatch goal with
   | X : reified_op
           _
           (PushButtonSynthesis.UnsaturatedSolinas.carry_mul _ _ _ _)
     |- _ =>
-    destruct X as [? carry_mul_func carry_mul_func_eq ]
+    destruct X as [? carry_mul_func_value carry_mul_func_eq ]
   end;
+  let name := eval vm_compute in carry_mul_name_value in
   apply Build_bedrock2_unsaturated_solinas
-    with (carry_mul:= (carry_mul_name, carry_mul_func));
+    with (carry_mul_name:=name)
+         (carry_mul_func:=carry_mul_func_value);
   rewrite carry_mul_func_eq.
 
 Module X25519_64.
@@ -145,7 +151,8 @@ Module X25519_64.
     all: try assumption.
     all: abstract (handle_easy_preconditions).
   Defined.
-  (* Eval cbv [carry_mul curve25519_bedrock2] in carry_mul. *)
+(* Eval cbv [carry_mul API.carry_mul_name carry_mul_func
+                      curve25519_bedrock2] in carry_mul. *)
 End X25519_64.
 
 Module X1305_32.
@@ -172,3 +179,132 @@ Module X1305_32.
     all: abstract (handle_easy_preconditions).
   Qed.
 End X1305_32.
+
+Require Import bedrock2.Array.
+Require Import bedrock2.Map.Separation.
+Require Import bedrock2.Map.SeparationLogic.
+Require Import Crypto.Arithmetic.Core.
+Require Import Crypto.Bedrock.Tactics.
+Require Import Crypto.COperationSpecifications.
+Require Import bedrock2.Semantics.
+Import Types.
+Module Test.
+  Import X25519_64.
+  Existing Instance Defaults64.default_parameters.
+  Existing Instance curve25519_bedrock2.
+  Local Open Scope string_scope.
+  Local Coercion name_of_func (f : bedrock_func) := fst f.
+
+  (* test function; computes x * y * y *)
+  Definition mul_twice : bedrock_func :=
+    let x := "x" in
+    let y := "y" in
+    let xy := "xy" in
+    let tmp := "tmp" in
+    let out := "out" in
+    ("mul_twice",
+     ([x; y; out], [],
+      (cmd.seq
+         (cmd.call [] "curve25519_carry_mul" [expr.var x; expr.var y; expr.var out])
+         (cmd.call [] "curve25519_carry_mul" [expr.var out; expr.var y; expr.var out])))).
+
+  (* Notations to make the spec more readable *)
+  Local Notation M := (X25519_64.s - Associational.eval X25519_64.c).
+  Local Notation eval :=
+    (Positional.eval
+                (weight X25519_64.n X25519_64.s X25519_64.c)
+                X25519_64.n).
+  Local Notation loose_bounds :=
+    (UnsaturatedSolinas.loose_bounds X25519_64.n X25519_64.s X25519_64.c).
+  Local Notation tight_bounds :=
+    (UnsaturatedSolinas.tight_bounds X25519_64.n X25519_64.s X25519_64.c).
+
+  Instance spec_of_mul_twice : spec_of mul_twice :=
+    fun functions =>
+      forall x y px py pout bs t m
+             (R : Interface.map.rep
+                    (map:=Semantics.mem) -> Prop),
+        list_Z_bounded_by loose_bounds x ->
+        list_Z_bounded_by loose_bounds y ->
+        length bs = (X25519_64.n * Z.to_nat word_size_in_bytes)%nat ->
+        (* all 3 need to be separate, because we use out as an input with y *)
+        sep (sep (Bignum px x)
+                 (sep (Bignum py y)
+                      (array ptsto (Interface.word.of_Z 1) pout bs)))
+            R m ->
+        WeakestPrecondition.call
+          (p:=Types.semantics)
+          functions mul_twice t m
+          (px :: py :: pout :: nil)
+          (fun t' m' rets =>
+             t = t' /\
+             rets = []%list /\
+             Lift1Prop.ex1
+               (fun out =>
+                  sep
+                    (sep (emp (eval out mod M
+                               = (eval x * eval y * eval y) mod M
+                               /\ list_Z_bounded_by tight_bounds out))
+                         (Bignum pout out))
+                    (sep (Bignum px x) (sep (Bignum py y) R))) m').
+
+  About spec_of_carry_mul.
+  Local Notation function_t := ((String.string * (list String.string * list String.string * Syntax.cmd.cmd))%type).
+  Local Notation functions_t := (list function_t).
+
+  (* TODO: currently this extra step is required so the literal string isn't
+  hidden *)
+  Instance spec_of_curve25519_carry_mul :
+    spec_of "curve25519_carry_mul" := spec_of_carry_mul.
+
+  Lemma mul_twice_correct :
+    program_logic_goal_for_function! mul_twice.
+  Proof.
+    (* first step of straightline is inlined here so we can do a [change]
+       instead of [replace] *)
+    enter mul_twice. intros.
+    WeakestPrecondition.unfold1_call_goal.
+    (cbv beta match delta [WeakestPrecondition.call_body]).
+    lazymatch goal with
+    | |- if ?test then ?T else _ =>
+      (* this change is a replace in the original straightline, but that hangs
+      here for some reason *)
+      change test with true; change_no_check T
+    end.
+    (cbv beta match delta [WeakestPrecondition.func]).
+
+    repeat straightline.
+    straightline_call;
+      [ try ecancel_assumption .. | ];
+      [ assumption .. | ].
+    sepsimpl.
+    repeat straightline.
+    straightline_call;
+      [ try ecancel_assumption .. | ].
+    { apply relax_correct; assumption. }
+    { assumption. }
+    { (* TODO: lemma about length of encode_bytes *)
+      admit. }
+    {
+      use_sep_assumption.
+      rewrite (Bignum_to_bytes
+                       (inname_gen:=inname_gen)
+                       (outname_gen:=outname_gen)) by
+          admit. (* currently has a million preconditions because admitted *)
+      ecancel. }
+
+    repeat straightline.
+
+    repeat split; try reflexivity.
+    sepsimpl_hyps.
+    eexists; sepsimpl;
+      [ | | ecancel_assumption ];
+      [ | assumption ].
+    repeat match goal with
+           | H : eval _ mod _ = (eval _ * eval _) mod _ |- _ =>
+             rewrite H
+           | _ => progress Modulo.push_Zmod
+           end.
+    reflexivity.
+  Admitted.
+End Test.
